src/Sound/Defs.dfy
@@ -1,0 +1,329 @@
+module Defs { 
+
+  datatype Except<+T> =
+    | Ok(res: T)
+    | Error
+  {
+    predicate IsFailure() {
+      Error?
+    }
+    function PropagateFailure<U>(): Except<U>
+      requires IsFailure()
+    {
+      Error
+    }
+    function Extract() : T 
+      requires !IsFailure()
+    {
+      res
+    }
+  }
+
+  function ExceptUpdate(e: Except<State>, v: Variable, b: bool): Except<State> {
+    var r :- e;
+    Ok(r.Update(v, b))
+  }
+
+  function ExceptRemove(e: Except<State>, v: Variable): Except<State> {
+    var r :- e;
+    Ok(r - {v})
+  }
+
+  // import opened Values
+
+  // class Variable
+  // {
+  //   const name: string
+
+  //   constructor (name: string) {
+  //     this.name := name;
+  //   }
+  // }
+  type Variable = string
+
+  datatype Expr =
+    | BConst(bvalue: bool)
+    | And(0: Expr, 1: Expr)
+    | Or(0: Expr, 1: Expr)
+    | Not(e: Expr)
+    | Implies(0: Expr, 1: Expr)
+    | Var(v: Variable)
+    | Forall(v: Variable, body: Expr) 
+  {
+    function FVars(): set<Variable> {
+      match this
+      case BConst(_) => {}
+      case And(e0, e1) => e0.FVars() + e1.FVars()
+      case Or(e0, e1) => e0.FVars() + e1.FVars()
+      case Not(e) => e.FVars()
+      case Implies(e0, e1) => e0.FVars() + e1.FVars()
+      case Forall(v, body) => body.FVars() - {v}
+      case Var(v) => {v}
+    }
+
+    function BVars(): set<Variable> {
+      match this
+      case BConst(_) => {}
+      case And(e0, e1) => e0.BVars() + e1.BVars()
+      case Or(e0, e1) => e0.BVars() + e1.BVars()
+      case Not(e) => e.BVars()
+      case Implies(e0, e1) => e0.BVars() + e1.BVars()
+      case Forall(v, body) => body.BVars() + {v}
+      case Var(v) => {}
+    }
+
+    predicate IsDefinedOn(s: set<Variable>) {
+      FVars() <= s
+    }
+
+    predicate NoShadowing() {
+      match this
+      case BConst(_) => true
+      case Var(v) => true
+      case And(e0, e1) => e0.NoShadowing() && e1.NoShadowing()
+      case Or(e0, e1) => e0.NoShadowing() && e1.NoShadowing()
+      case Not(e) => e.NoShadowing()
+      case Implies(e0, e1) => e0.NoShadowing() && e1.NoShadowing()
+      case Forall(v, body) => v !in body.BVars() && body.NoShadowing()
+    }
+
+    predicate WellFormed() {
+      NoShadowing()
+    }
+    
+    lemma IsDefinedOnTransitivity(s1: set<Variable>, s2: set<Variable>)
+        requires s1 <= s2
+        ensures IsDefinedOn(s1) ==> IsDefinedOn(s2)
+    {  }
+
+    ghost predicate Holds() {
+      forall s: State :: IsDefinedOn(s.Keys) ==> s.Eval(this)
+    }
+
+    lemma EvalFVarsLemma(s1: State, s2: State) 
+      requires IsDefinedOn(s1.Keys)
+      requires IsDefinedOn(s2.Keys)
+      requires forall v: Variable :: v in FVars() ==> s1[v] == s2[v]
+      ensures s1.Eval(this) == s2.Eval(this)
+
+    { 
+      match this
+      case Forall(v, body) => 
+        forall x: bool { 
+          body.EvalFVarsLemma(s1.Update(v, x), s2.Update(v, x)); 
+        }
+      case _ =>
+    }
+      
+  }
+
+  function Eq(e1: Expr, e2: Expr): Expr {
+    And(Implies(e1, e2), Implies(e2, e1))
+  }
+
+  lemma FVarsEqLemma(e1: Expr, e2: Expr)
+    ensures Eq(e1, e2).FVars() == e1.FVars() + e2.FVars()
+  {  }
+
+  lemma EvalEqLemma(e1: Expr, e2: Expr, s: State)
+    requires e1.IsDefinedOn(s.Keys)
+    requires e2.IsDefinedOn(s.Keys)
+    requires s.Eval(e1) == s.Eval(e2)
+    ensures s.Eval(Eq(e1, e2))
+  {  }
+    
+  datatype Stmt =
+    | Check(e: Expr)
+    | Assume(e: Expr)
+    | Seq(ss: seq<Stmt>)
+    | Assign(lhs: Variable, rhs: Expr)
+    | VarDecl(v: Variable, s: Stmt)
+    // | While(guard: Expr, inv: Expr, body: Stmt)
+    | Choice(0: Stmt, 1: Stmt)
+  {
+    function Size(): nat {
+      match this
+      case Check(_) => 1
+      case Assume(_) => 1
+      case Seq(ss) => 1 + SeqSize(ss)
+      case Assign(_, _) => 1
+      case Choice(s0, s1) => 1 + s0.Size() + s1.Size()
+      case VarDecl(_, s) => 1 + s.Size()
+    }
+
+    function FVars(): set<Variable> {
+      match this
+      case Check(e) => e.FVars()
+      case Assume(e) => e.FVars()
+      case Seq(ss) => SeqFVars(ss)
+      case Assign(lhs, rhs) => {lhs} + rhs.FVars()
+      case VarDecl(v, s) => s.FVars() - {v}
+      case Choice(s0, s1) => s0.FVars() + s1.FVars()
+    }
+
+    function BVars(): set<Variable> {
+      match this
+      case Check(e) => e.BVars()
+      case Assume(e) => e.BVars()
+      case Seq(ss) => SeqBVars(ss)
+      case Assign(lhs, rhs) => rhs.BVars()
+      case VarDecl(v, s) => s.BVars() + {v}
+      case Choice(s0, s1) => s0.BVars() + s1.BVars()
+    }
+
+    predicate NoShadowing() {
+      match this
+      case Check(e) => e.NoShadowing()
+      case Assume(e) => e.NoShadowing()
+      case Seq(ss) => SeqNoShadowing(ss, this)
+        // && SeqNoShadowingNested(ss)
+        // && (forall i, j :: 0 <= i < j < |ss| ==> ss[i].BVars() !* ss[j].BVars())
+      case Assign(lhs, rhs) => rhs.NoShadowing()
+      case VarDecl(v, s) => v !in s.BVars() && s.NoShadowing()
+      case Choice(s0, s1) => s0.NoShadowing() && s1.NoShadowing()
+    }
+
+    predicate WellFormed() {
+      NoShadowing() && FVars() !! BVars()
+    }
+
+    predicate IsDefinedOn(s: set<Variable>) {
+      FVars() <= s
+    }
+    lemma IsDefinedOnTransitivity(s1: set<Variable>, s2: set<Variable>)
+      requires s1 <= s2
+      ensures IsDefinedOn(s1) ==> IsDefinedOn(s2)
+    {  }
+
+    predicate Single() {
+      match this
+      case Assign(_, _) => true
+      case Check(_) => true
+      case Assume(_) => true
+      case _ => false
+    }
+  }
+
+  function SeqSize(ss: seq<Stmt>): nat {
+    if ss == [] then 0 else ss[0].Size() + SeqSize(ss[1..])
+  }
+
+  lemma SeqSizeSplitLemma(ss: seq<Stmt>)
+    requires ss != []
+    ensures SeqSize(ss) == ss[0].Size() + SeqSize(ss[1..])
+  {  }
+
+  function SeqFVars(ss: seq<Stmt>): set<Variable> 
+    decreases ss
+  {
+    if ss == [] then {} else ss[0].FVars() + SeqFVars(ss[1..])
+  }
+
+  function SeqBVars(ss: seq<Stmt>): set<Variable> {
+    if ss == [] then {} else ss[0].BVars() + SeqBVars(ss[1..])
+  }
+
+  function Conj(ctx: seq<Expr>): Expr 
+  {
+    if ctx == [] then BConst(true) else And(ctx[0], Conj(ctx[1..]))
+  }
+
+  lemma ConjFVarsMonotonicity(ctx1: seq<Expr>, ctx2: seq<Expr>)
+    requires ctx1 <= ctx2
+    ensures Conj(ctx1).FVars() <= Conj(ctx2).FVars()
+  {  }
+
+  lemma FVarsConjUnionLemma(ctx1: seq<Expr>, ctx2: seq<Expr>)
+    ensures Conj(ctx1 + ctx2).FVars() == Conj(ctx1).FVars() + Conj(ctx2).FVars()
+  {
+    if ctx1 == [] {
+      assert [] + ctx2 == ctx2;
+    } else {
+      assert ctx1 + ctx2 == [ctx1[0]] + (ctx1[1..] + ctx2);
+    }
+  }
+
+  predicate SeqIsDefinedOn(ss: seq<Stmt>, s: set<Variable>) 
+    ensures SeqIsDefinedOn(ss, s) <==> SeqFVars(ss) <= s
+  {
+    if ss == [] then true else ss[0].IsDefinedOn(s) && SeqIsDefinedOn(ss[1..], s)
+  }
+
+  lemma IsDefinedOnAndLemma(e0: Expr, e1: Expr, s: State)
+    requires e0.IsDefinedOn(s.Keys) && e1.IsDefinedOn(s.Keys)
+    ensures And(e0, e1).IsDefinedOn(s.Keys) { }
+
+  lemma IsDefinedOnConjLemma(ctx: seq<Expr>, s: State)
+    requires forall e <- ctx :: e.IsDefinedOn(s.Keys)
+    ensures Conj(ctx).IsDefinedOn(s.Keys)
+    {
+      if ctx != [] { IsDefinedOnAndLemma(ctx[0], Conj(ctx[1..]), s); }
+    }
+
+  lemma EvalConjLemma(ctx: seq<Expr>, s: State)
+    requires forall e <- ctx :: e.IsDefinedOn(s.Keys)
+    requires forall e <- ctx :: s.Eval(e)
+    ensures (IsDefinedOnConjLemma(ctx, s); s.Eval(Conj(ctx)))
+  {  }
+
+  predicate SeqNoShadowingNested(ss: seq<Stmt>, ghost parent: Stmt := Seq(ss)) 
+    requires forall s <- ss :: s < parent
+    decreases parent, |ss|
+  {
+    forall s <- ss :: s.NoShadowing()
+  }
+
+  predicate SeqNoShadowing(ss: seq<Stmt>, ghost parent: Stmt := Seq(ss)) 
+    requires forall s <- ss :: s < parent
+    decreases parent, |ss| + 1
+  {
+    && SeqNoShadowingNested(ss, parent)
+    && (forall i, j :: 0 <= i < j < |ss| ==> ss[i].BVars() !! ss[j].BVars())
+  }
+
+  predicate SeqWellFormed(ss: seq<Stmt>) {
+    if ss == [] then 
+      true 
+    else 
+      && ss[0].WellFormed()
+      && ss[0].BVars() !! SeqFVars(ss[1..]) 
+      && ss[0].BVars() !! SeqBVars(ss[1..])
+      && SeqWellFormed(ss[1..])
+  }
+
+  lemma SeqFunConcatLemmas(ss1: seq<Stmt>, ss2: seq<Stmt>)
+    ensures SeqSize(ss1 + ss2) == SeqSize(ss1) + SeqSize(ss2)
+    ensures SeqBVars(ss1 + ss2) == SeqBVars(ss1) + SeqBVars(ss2)
+    ensures SeqFVars(ss1 + ss2) == SeqFVars(ss1) + SeqFVars(ss2)
+  {
+    if ss1 == [] {
+      assert ss1 + ss2 == ss2;
+    } else {
+      assert (ss1 + ss2)[0] == ss1[0];
+      assert (ss1 + ss2)[1..] == ss1[1..] + ss2;
+    }
+  }
+
+  type Value = bool
+
+  newtype State = map<Variable, Value> {
+    
+    function Eval(e: Expr): Value 
+      requires e.IsDefinedOn(this.Keys)
+      decreases e
+    {
+      match e
+      case BConst(bvalue) => bvalue
+      case And(e0, e1) => Eval(e0) && Eval(e1)
+      case Or(e0, e1) => Eval(e0) || Eval(e1)
+      case Not(e) => !Eval(e)
+      case Implies(e0, e1) => Eval(e0) ==> Eval(e1)
+      case Forall(v, body) => forall x: bool :: Update(v, x).Eval(body)
+      case Var(v) => this[v]
+    }
+    function Update(v: Variable, val: Value): State {
+      this[v := val]
+    }
+  }
+}
+
