src/Sound/VCGen/Omni.dfy
@@ -1,0 +1,79 @@
+module VCGenOmni {
+  import opened Defs
+  import opened Context
+  import Omni
+  import WellFormed
+
+  ghost const AllStates: iset<State> := iset st: State | true
+
+  method VCGen(s: Stmt, context_in: Context) returns (context: Context, VCs: seq<Expr>) 
+    requires s.BVars() <= context_in.bVars
+    requires s.IsDefinedOn(context_in.incarnation.Keys)
+    requires context_in.Valid()
+    requires s.Single()
+    requires s.IsDefinedOn(context_in.incarnation.Keys)
+
+    ensures context.Valid()
+    ensures context_in.bVars == context.bVars
+    ensures context_in.incarnation.Keys <= context.incarnation.Keys
+    ensures (forall e <- VCs :: e.Holds()) ==> 
+      forall st: State :: 
+        context_in.IsSatisfiedOn(st) ==>
+        Omni.Sem(s, context_in.AdjustState(st), context_in.AdjustedModels)
+  {
+    context := context_in;
+    match s
+    case Check(e) =>
+      VCs := [context_in.MkEntailment(e)];
+    case Assume(e) =>
+      context := context_in.Add(e);
+      VCs := [];
+    case Assign(v, x) =>
+      ghost var vNew;
+      vNew, context := context_in.AddEq(v, x);
+      VCs := [];
+  }
+
+method SeqVCGen(s: seq<Stmt>, context: Context) returns (VCs: seq<Expr>) 
+  requires SeqWellFormed(s)
+  requires SeqBVars(s) <= context.bVars
+  requires SeqIsDefinedOn(s, context.incarnation.Keys)
+
+  requires context.Valid()
+  decreases SeqSize(s)
+  ensures
+    (forall e <- VCs :: e.Holds()) ==> 
+      forall st: State:: 
+        context.IsSatisfiedOn(st) ==> Omni.SeqSem(s, context.AdjustState(st), AllStates)
+  {
+    if s == [] { 
+      VCs := []; 
+      return; 
+    }
+    var stmt, cont := s[0], s[1..];
+    assert s == [stmt] + cont;
+    SeqSizeSplitLemma(s);
+    if stmt.Single() {
+      var VCstmt, VCcont, context';
+      context', VCstmt := VCGen(stmt, context);
+      VCcont := SeqVCGen(cont, context');
+      VCs := VCstmt + VCcont;
+    } else {
+      match stmt 
+      case Seq(ss) =>
+        SeqFunConcatLemmas(ss, cont);
+        WellFormed.SeqLemma(ss, cont);
+        VCs := SeqVCGen(ss + cont, context);
+      case Choice(ss0, ss1) =>
+        var VCs0 := SeqVCGen([ss0] + cont, context);
+        var VCs1 := SeqVCGen([ss1] + cont, context);
+        VCs := VCs0 + VCs1;
+      case VarDecl(v, s) =>
+        ghost var vNew;
+        var context';
+        vNew, context' := context.AddVar(v);
+        VCs := SeqVCGen([s] + cont, context');
+      case _ => assume {:axiom} false;
+    }
+  }
+}
